Parser.v
@@ -28,7 +28,7 @@ Module ParserFn (Import D : Defs.T).
                           | Reject : string -> parse_result
                           | Error  : parse_error -> parse_result.
 
-  Definition step (g      : grammar)
+  Definition step (g : grammar)
              (p_stk  : prefix_stack)
              (s_stk  : suffix_stack)
              (ts     : list token)
@@ -440,5 +440,137 @@ Module ParserFn (Import D : Defs.T).
     let p_stk0 := (PF [] [], []) in
     let s_stk0 := (SF gamma, []) in
     multistep g p_stk0 s_stk0 ts (allNts g) true (lex_nat_triple_wf _). 
+
+  (* cache-optimized version *)
+
+  Inductive step_result_opt :=
+  | StepAccept_opt : forest -> step_result_opt
+  | StepReject_opt : string -> step_result_opt
+  | StepK_opt      : prefix_stack -> suffix_stack -> list token -> NtSet.t -> bool -> cache -> step_result_opt
+  | StepError_opt  : parse_error -> step_result_opt.
+
+  Definition step_opt (g      : grammar)
+                      (p_stk  : prefix_stack)
+                      (s_stk  : suffix_stack)
+                      (ts     : list token)
+                      (av     : NtSet.t)
+                      (u      : bool) 
+                      (c      : cache) : step_result_opt := 
+    match p_stk, s_stk with
+    | (PF pre v, p_frs), (SF suf, s_frs) =>
+      match suf with
+      (* no more symbols to process in current frame *)
+      | [] =>
+        match p_frs, s_frs with
+        (* empty stacks --> terminate *)
+        | [], [] => 
+          match ts with
+          | []     => StepAccept_opt (rev v)
+          | _ :: _ => StepReject_opt "stack exhausted, tokens remain"
+          end
+        (* nonempty stacks --> return to caller frames *)
+        | PF pre_cr v_cr :: p_frs', SF suf_cr :: s_frs' =>
+          match suf_cr with
+          | []                => StepError_opt InvalidState
+          | T _  :: _         => StepError_opt InvalidState
+          | NT x :: suf_cr'   =>
+            let p_stk' := (PF (NT x :: pre_cr) (Node x (rev v) :: v_cr), p_frs') in
+            let s_stk' := (SF suf_cr', s_frs')                                   in
+            StepK_opt p_stk' s_stk' ts (NtSet.add x av) u c
+          end
+        | _, _ => StepError_opt InvalidState
+        end
+      (* terminal case --> consume a token *)
+      | T a :: suf' =>
+        match ts with
+        | []             => StepReject_opt "input exhausted"
+        | (a', l) :: ts' =>
+          if t_eq_dec a' a then
+            let p_stk' := (PF (T a :: pre) (Leaf a l :: v), p_frs) in
+            let s_stk' := (SF suf', s_frs)                         in
+            StepK_opt p_stk' s_stk' ts' (allNts g) u c
+          else
+            StepReject_opt "token mismatch"
+        end
+      (* nonterminal case --> push a frame onto the stack *)
+      | NT x :: _ => 
+        if NtSet.mem x av then
+          match adaptivePredict g x s_stk ts c with
+          | (c', PredSucc rhs) =>
+            let p_stk' := (PF [] [], PF pre v :: p_frs) in
+            let s_stk' := (SF rhs, SF suf :: s_frs)     in
+            StepK_opt p_stk' s_stk' ts (NtSet.remove x av) u c'
+          | (c', PredAmbig rhs) =>
+            let p_stk' := (PF [] [], PF pre v :: p_frs) in
+            let s_stk' := (SF rhs, SF suf :: s_frs)     in
+            StepK_opt p_stk' s_stk' ts (NtSet.remove x av) false c'
+          | (_, PredReject) =>
+            StepReject_opt "prediction found no viable right-hand sides"
+          | (_, PredError e) =>
+            StepError_opt (PredictionError e)
+          end
+        else if NtSet.mem x (allNts g) then
+               StepError_opt (LeftRecursion x)
+             else
+               StepReject_opt "nonterminal not in grammar"
+      end
+    end.
+    
+    (* 
+  Lemma step_meas_lt_opt :
+    forall g p_stk p_stk' s_stk s_stk' ts ts' av av' u u' c c',
+      step_opt g p_stk s_stk ts av u c = StepK_opt p_stk' s_stk' ts' av' u' c'
+      -> lex_nat_triple (meas g s_stk' ts' av') (meas g s_stk ts av).
+  Proof.
+    intros g pstk pstk' sstk stk' ts ts' av av' u u' c c' hs; unfold step_opt in hs.
+    destruct sstk as ([ [| [a|x] suf] ], frs).
+    - dms; tc; inv hs.
+      eapply meas_lt_after_return; eauto.
+    - dms; tc; inv hs.
+      apply triple_fst_lt; auto.
+    - destruct pstk as ([pre v], p_frs).
+      destruct (NtSet.mem x av) eqn:hm; [.. | dms; tc].
+      apply NtSet.mem_spec in hm.
+      destruct (llPredict _ _ _ _) eqn:hp; dms; tc; inv hs.
+      + apply llPredict_succ_in_grammar in hp.
+        eapply meas_lt_after_push; eauto.
+      + apply llPredict_ambig_in_grammar in hp.
+        eapply meas_lt_after_push; eauto.
+  Qed.
+     *)
+    
+  Axiom magic : forall A, A.
+    
+  Lemma StepK_result_acc_opt :
+    forall g ps ps' ss ss' ts ts' av av' u u' c c' (a : Acc lex_nat_triple (meas g ss ts av)),
+      step_opt g ps ss ts av u c = StepK_opt ps' ss' ts' av' u' c'
+      -> Acc lex_nat_triple (meas g ss' ts' av').
+  Proof.
+    intros; eapply Acc_inv; eauto.
+    apply magic.
+  Defined.
+  
+  Fixpoint multistep_opt (g  : grammar)
+                         (ps : prefix_stack)
+                         (ss : suffix_stack)
+                         (ts : list token)
+                         (av : NtSet.t)
+                         (u  : bool)
+                         (c  : cache)
+                         (a  : Acc lex_nat_triple (meas g ss ts av))
+                         {struct a} : parse_result :=
+    match step_opt g ps ss ts av u c as res return step_opt g ps ss ts av u c = res -> _ with
+    | StepAccept_opt v             => fun _  => if u then Accept v else Ambig v
+    | StepReject_opt s             => fun _  => Reject s
+    | StepError_opt e              => fun _  => Error e
+    | StepK_opt ps' ss' ts' av' u' c' =>
+      fun hs => multistep_opt g ps' ss' ts' av' u' c'
+                              (StepK_result_acc_opt _ _ _ _ _ _ _ _ _ _ _ _ _ a hs)
+    end eq_refl.
+  
+  Definition parse_opt (g : grammar) (gamma : list symbol) (ts : list token) : parse_result :=
+    let p_stk0 := (PF [] [], []) in
+    let s_stk0 := (SF gamma, []) in
+    multistep_opt g p_stk0 s_stk0 ts (allNts g) true (Cache.empty (list subparser)) (lex_nat_triple_wf _). 
 
 End ParserFn.
